examples/hkt-dict-parametricity.tig.lisp
@@ -3,28 +3,28 @@
 let i_Functor_0 : ∀a, Functor (Sum a) =
   Λ a.
     Functor@(Sum a)
-      Λ a b.
-        fun f : a → b =>
-          fun ?x₀ : Sum a a =>
+      Λ a₁ b.
+        fun f : a₁ → b =>
+          fun ?x₀ : Sum a a₁ =>
             match ?x₀ with
             | Inl a => Inl@a@b a
             | Inr b => Inr@a@b (f b)
 
-let main : ∀α[Functor (Sum α)], Sum Int Int × Sum α Int =
+let main : ∀α [Functor (Sum α)], Sum Int Int × Sum α Int =
   Λ α.
     let rd_Functor_0 : Functor (Sum Int) = i_Functor_0@Int
     in fun d_Functor_0 : Functor (Sum α) =>
-      let a : ∀α, Sum Int α = Λ α. Inl@Int@α 2
-      and b : ∀α, Sum α Int = Λ α. Inr@α@Int 1
+      let a : ∀β, Sum Int β = Λ β. Inl@Int@β 2
+      and b : ∀γ, Sum γ Int = Λ γ. Inr@γ@Int 1
       in ⟨rd_Functor_0[0, fmap]@(Sum Int) fun ?x₀ : Int => mul 2 ?x₀ a@Int,
           d_Functor_0[0, fmap]@(Sum α) fun ?x₀ : Int => add 1 ?x₀ b@α⟩
 ;; == TCNF IR ==
 
 let i_Functor_0#2/0 : Functor (Sum a) =
-  let fn#3 (f#4 : a → b, ?x₀#5 : Sum a a) : (a → b) → Sum a a → Sum a b =
+  let fn#3 (f#4 : a₁ → b, ?x₀#5 : Sum a a₁) : (a₁ → b) → Sum a a₁ → Sum a b =
     case #5 of
       Inl⟦f#6 : a⟧ => let con#7 : Sum a b = Inl⟦#6⟧; ret #7;
-      Inr⟦f#8 : a⟧ =>
+      Inr⟦f#8 : a₁⟧ =>
         let app#9 : b = #4(#8); let con#10 : Sum a b = Inr⟦#9⟧; ret #10;
       _ => (⊥ : Sum a b);
   let con#11 : Functor (Sum a) = Functor⟦#3⟧; ret #11
@@ -32,24 +32,24 @@ let i_Functor_0#2/0 : Functor (Sum a) =
 let main#12/0 : Functor (Sum α) → Sum Int Int × Sum α Int =
   let fn#13 (d_Functor_0#14 : Functor (Sum α))
     : Functor (Sum α) → Sum Int Int × Sum α Int =
-    let con#15 : Sum Int α = Inl⟦2⟧;
-    let con#16 : Sum α Int = Inr⟦1⟧;
-    let pr#17 : (a → b) → Sum Int a → Sum Int b = #2@Functor[0];
+    let con#15 : Sum Int β = Inl⟦2⟧;
+    let con#16 : Sum γ Int = Inr⟦1⟧;
+    let pr#17 : (?m.3 → ?m.4) → Sum Int ?m.3 → Sum Int ?m.4 = #2@Functor[0];
     let fn#18 (?x₀#19 : Int) : Int → Int =
       let π#20 : Int = MUL(2, #19); ret #20;
-    let app#21 : Sum Int b = #17(#18, #15);
-    let pr#22 : (a → b) → Sum α a → Sum α b = #14@Functor[0];
+    let app#21 : Sum Int ?m.4 = #17(#18, #15);
+    let pr#22 : (?m.3 → ?m.4) → Sum α ?m.3 → Sum α ?m.4 = #14@Functor[0];
     let fn#23 (?x₀#24 : Int) : Int → Int =
       let π#25 : Int = ADD(1, #24); ret #25;
-    let app#26 : Sum α b = #22(#23, #16);
+    let app#26 : Sum α ?m.4 = #22(#23, #16);
     let p#27 : Sum Int Int × Sum α Int = ⟨#21, #26⟩; ret #27;
   ret #13
 ;; == TCNF CC & Optimize'd ==
 
-let fn#28/2 (f#4 : a → b, ?x₀#5 : Sum a a) : (a → b) → Sum a a → Sum a b =
+let fn#28/2 (f#4 : a₁ → b, ?x₀#5 : Sum a a₁) : (a₁ → b) → Sum a a₁ → Sum a b =
   case #5 of
     Inl⟦f#6 : a⟧ => let con#7 : Sum a b = Inl⟦#6⟧; ret #7;
-    Inr⟦f#8 : a⟧ =>
+    Inr⟦f#8 : a₁⟧ =>
       let app#9 : b = #4(#8); let con#10 : Sum a b = Inr⟦#9⟧; ret #10;
     _ => (⊥ : Sum a b)
 
@@ -59,16 +59,16 @@ let fn#31/1 (?x₀#24 : Int) : Int → Int = let π#25 : Int = ADD(1, #24); ret 
 
 let fn#29/1 (d_Functor_0#14 : Functor (Sum α))
   : Functor (Sum α) → Sum Int Int × Sum α Int =
-  let con#15 : Sum Int α = Inl⟦2⟧;
-  let con#16 : Sum α Int = Inr⟦1⟧;
+  let con#15 : Sum Int β = Inl⟦2⟧;
+  let con#16 : Sum γ Int = Inr⟦1⟧;
   let fn#18 : Int → Int = 𝐂⟦30⟧;
-  let app#21 : Sum Int b = #28(#18, #15);
+  let app#21 : Sum Int ?m.4 = #28(#18, #15);
   let fn#23 : Int → Int = 𝐂⟦31⟧;
-  let app#26 : Sum α b = #14(#23, #16);
+  let app#26 : Sum α ?m.4 = #14(#23, #16);
   let p#27 : Sum Int Int × Sum α Int = ⟨#21, #26⟩; ret #27
 
 let i_Functor_0#2/0 : Functor (Sum a) =
-  let fn#3 : (a → b) → Sum a a → Sum a b = 𝐂⟦28⟧; ret #3
+  let fn#3 : (a₁ → b) → Sum a a₁ → Sum a b = 𝐂⟦28⟧; ret #3
 
 let main#12/0 : Functor (Sum α) → Sum Int Int × Sum α Int =
   let fn#13 : Functor (Sum α) → Sum Int Int × Sum α Int = 𝐂⟦29⟧; ret #13
