examples/poly-ref-io.tig.lisp
@@ -1,5 +1,156 @@
+;; == System F IR ==
+
+let mkref : ∀a, a → IO (Ref a) = Λ a. quote
+
+let deref : ∀a, Ref a → IO a = Λ a. eval
+
+let setf : ∀a, Ref a → a → IO Unit = Λ a. set
+
+let pureIO : ∀a, a → IO a = Λ a. identity
+
+let unsafeIO : ∀a, IO a → a = Λ a. identity
+
+let (::) : ∀α, α → List α → List α = Λ α. Cons@α
+
+let (>>=) : ∀α [Monad α], ∀a b, α a → (a → α b) → α b =
+  Λ α. fun d_Monad_0 : Monad α => Λ a b. d_Monad_0[1, bind]@α
+
+let (ₚ') : ∀α, α → IO (Ref α) = Λ α. mkref@α
+
+let i_Monad_0 : Monad IO =
+  Monad@IO Λ a. pureIO@a
+    Λ a₁ b. fun act : IO a₁ => fun f : a₁ → IO b => f (unsafeIO@a₁ act)
+
+let ioref : ∀α, IO (Ref (List α)) = Λ α. mkref@(List α) Nil@α
+
+let f : ∀α, α → IO Unit =
+  Λ α.
+    rec fun f : α → IO Unit =>
+      fun _ : α =>
+        let rd_Monad_0 : Monad IO = i_Monad_0
+        in rd_Monad_0[1, bind]@IO ioref@Int
+             fun ref : Ref (List Int) =>
+               setf@(List Int) ref (Cons@Int 1 Nil@Int)
+and g : ∀α, α → IO Bool =
+  Λ α.
+    rec fun g : α → IO Bool =>
+      fun _ : α =>
+        let rd_Monad_0 : Monad IO = i_Monad_0
+        in rd_Monad_0[1, bind]@IO ioref@?m.62
+             fun ref : Ref (List ?m.62) =>
+               rd_Monad_0[1, bind]@IO (deref@(List ?m.62) ref)
+                 fun ?x₀ : List ?m.62 =>
+                   match ?x₀ with
+                   | Nil => rd_Monad_0[0, pure]@IO true
+and main : IO Bool = let _ : IO Unit = f@Unit () in g@Unit ()
+;; == TCNF IR ==
+
+let mkref#2/1 (η#3 : a) : a → IO (Ref a) =
+  let ffi#4 : IO (Ref a) = @quote(#3); ret #4
+
+let deref#5/1 (η#6 : Ref a) : Ref a → IO a =
+  let ffi#7 : IO a = @eval(#6); ret #7
+
+let setf#8/2 (η#9 : Ref a, η#10 : a) : Ref a → a → IO Unit =
+  let ffi#11 : IO Unit = @set(#9, #10); ret #11
+
+let pureIO#12/1 (η#13 : a) : a → IO a =
+  let ffi#14 : IO a = @identity(#13); ret #14
+
+let unsafeIO#15/1 (η#16 : IO a) : IO a → a =
+  let ffi#17 : a = @identity(#16); ret #17
+
+let i_Monad_0#18/0 : Monad IO =
+  let fn#19 (act#20 : IO a₁, f#21 : a₁ → IO b) : IO a₁ → (a₁ → IO b) → IO b =
+    let app#22 : a₁ = #15(#20); let app#23 : IO b = #21(#22); ret #23;
+  let con#24 : Monad IO = Monad⟦#12, #19⟧; ret #24
+
+let ioref#25/0 : IO (Ref (List α)) =
+  let con#26 : List α = Nil⟦⟧; let app#27 : IO (Ref (List α)) = #2(#26); ret #27
+
+let rec f#28/1 (_#30 : α) : α → IO Unit =
+  let pr#31 : IO ?m.10 → (?m.10 → IO ?m.11) → IO ?m.11 = #18@Monad[1];
+  let fn#32 (ref#33 : Ref (List Int)) : Ref (List Int) → IO Unit =
+    let con#34 : List Int = Nil⟦⟧;
+    let con#35 : List Int = Cons⟦1, #34⟧;
+    let app#36 : IO Unit = #8(#33, #35); ret #36;
+  let app#37 : IO ?m.11 = #31(#25, #32); ret #37
+
+let rec g#29/1 (_#38 : α) : α → IO Bool =
+  let pr#39 : IO ?m.10 → (?m.10 → IO ?m.11) → IO ?m.11 = #18@Monad[1];
+  let fn#40 (ref#41 : Ref (List ?m.62)) : Ref (List ?m.62) → IO Bool =
+    let pr#42 : IO ?m.10 → (?m.10 → IO ?m.11) → IO ?m.11 = #18@Monad[1];
+    let app#43 : IO (List ?m.62) = #5(#41);
+    let fn#44 (?x₀#45 : List ?m.62) : List ?m.62 → IO Bool =
+      join fail#46 : IO Bool = let fail#47 : IO Bool = #0(#45); ret #47;
+      case #45 of
+        Nil =>
+          let pr#48 : ?m.9 → IO ?m.9 = #18@Monad[0];
+          let app#49 : IO ?m.9 = #48(true); ret #49;
+        _ => jump #46();
+    let app#50 : IO ?m.11 = #42(#43, #44); ret #50;
+  let app#51 : IO ?m.11 = #39(#25, #40); ret #51
+
+let main#52/0 : IO Bool =
+  let app#53 : IO Unit = #28(()); let app#54 : IO Bool = #29(()); ret #54
+;; == TCNF CC & Optimize'd ==
+
+let fn#55/2 (act#20 : IO a₁, f#21 : a₁ → IO b) : IO a₁ → (a₁ → IO b) → IO b =
+  let app#22 : a₁ = #15(#20); let app#23 : IO b = #21(#22); ret #23
+
+let fn#56/1 (ref#33 : Ref (List Int)) : Ref (List Int) → IO Unit =
+  let con#34 : List Int = Nil⟦⟧;
+  let con#35 : List Int = Cons⟦1, #34⟧;
+  let app#36 : IO Unit = #8(#33, #35); ret #36
+
+let fn#58/1 (?x₀#45 : List ?m.62) : List ?m.62 → IO Bool =
+  join fail#46 : IO Bool = let fail#47 : IO Bool = #0(#45); ret #47;
+  case #45 of Nil => let app#49 : IO ?m.9 = #12(true); ret #49; _ => jump #46()
+
+let fn#57/1 (ref#41 : Ref (List ?m.62)) : Ref (List ?m.62) → IO Bool =
+  let app#43 : IO (List ?m.62) = #5(#41);
+  let fn#44 : List ?m.62 → IO Bool = 𝐂⟦58⟧;
+  let app#50 : IO ?m.11 = #55(#43, #44); ret #50
+
+let mkref#2/1 (η#3 : a) : a → IO (Ref a) =
+  let ffi#4 : IO (Ref a) = @quote(#3); ret #4
+
+let deref#5/1 (η#6 : Ref a) : Ref a → IO a =
+  let ffi#7 : IO a = @eval(#6); ret #7
+
+let setf#8/2 (η#9 : Ref a, η#10 : a) : Ref a → a → IO Unit =
+  let ffi#11 : IO Unit = @set(#9, #10); ret #11
+
+let pureIO#12/1 (η#13 : a) : a → IO a =
+  let ffi#14 : IO a = @identity(#13); ret #14
+
+let unsafeIO#15/1 (η#16 : IO a) : IO a → a =
+  let ffi#17 : a = @identity(#16); ret #17
+
+let i_Monad_0#18/0 : Monad IO =
+  let fn#19 : IO a₁ → (a₁ → IO b) → IO b = 𝐂⟦55⟧;
+  let con#24 : Monad IO = Monad⟦#12, #19⟧; ret #24
+
+let ioref#25/0 : IO (Ref (List α)) =
+  let con#26 : List α = Nil⟦⟧; let app#27 : IO (Ref (List α)) = #2(#26); ret #27
+
+let rec f#28/1 (_#30 : α) : α → IO Unit =
+  let fn#32 : Ref (List Int) → IO Unit = 𝐂⟦56⟧;
+  let app#37 : IO ?m.11 = #55(#25, #32); ret #37
+
+let rec g#29/1 (_#38 : α) : α → IO Bool =
+  let fn#40 : Ref (List ?m.62) → IO Bool = 𝐂⟦57⟧;
+  let app#51 : IO ?m.11 = #55(#25, #40); ret #51
+
+let main#52/0 : IO Bool =
+  let app#53 : IO Unit = #28(()); let app#54 : IO Bool = #29(()); ret #54
+;; == Runtime ==
+(load "runtime.lisp")
+
 ;; == Linked Lisp Source ==
 (load "ffi.lisp")
+
+;; == Common Lisp ==
 
 ; Prelude
 (declaim (optimize (speed 3) (safety 0) (debug 0)))
